Add cnot_commutes_through_phase_gadget

src/DiagramRules/PhaseGadgets.v
@@ -2,6 +2,7 @@ Require Import CoreData.
 Require Import CoreData.QlibTemp.
 Require Import CoreRules.
 Require Import Gates.
+Require Import Ingest.
 Require Import QuantumLib.Quantum.
 
 Global Open Scope ZX_scope.
@@ -17,7 +18,7 @@ Definition Z_phase_gadget (n : nat) (α : R) : ZX n n :=
   | (S n') => Z_phase_gadget_construct n' α
   end.
     
-Lemma Z_phase_gadget_fusion : forall α β n, Z_phase_gadget n α ⟷ Z_phase_gadget n β ∝ (Z_phase_gadget n (α + β)).
+Lemma Z_phase_gadget_full_fusion : forall α β n, Z_phase_gadget n α ⟷ Z_phase_gadget n β ∝ (Z_phase_gadget n (α + β)).
 Proof.
   intros.
   destruct n; [ simpl; cleanup_zx; easy | ].
@@ -46,7 +47,6 @@ Proof.
     easy.
 Qed.
 
-
 Inductive pauli_op : Type :=
   | PauliX
   | PauliY
@@ -58,6 +58,19 @@ Definition pauli_op_diag (op : pauli_op) : ZX 1 1 :=
   | PauliY => X 1 1 (PI / 2)
   | PauliZ => —
   end.
+
+Definition pauli_op_adj (op : pauli_op) : ZX 1 1 :=
+  match op with
+  | PauliX => □
+  | PauliY => X 1 1 (- (PI / 2))
+  | PauliZ => —
+  end.
+
+Lemma pauli_op_adj_is_adj : forall (op : pauli_op), (pauli_op_diag op)† ∝ pauli_op_adj op.
+Proof. 
+  intros. 
+  destruct op; easy.
+Qed.
 
 Lemma pauli_op_diag_unitary : forall op, unitary (pauli_op_diag op).
 Proof.
@@ -77,7 +90,7 @@ Definition pauli_str := list pauli_op.
 Fixpoint U (str : pauli_str) : ZX (length str) (length str) :=
   match str with
   | [] => ⦰
-  | hd :: tl => (pauli_op_to_ZX hd) ↕ (U tl)
+  | hd :: tl => (pauli_op_diag hd) ↕ (U tl)
   end.
 
 (* @nocheck name *)
@@ -115,8 +128,215 @@ Proof.
   cleanup_zx.
   apply compose_simplify; [ | easy].
   rewrite ComposeRules.compose_assoc.
-  rewrite Z_phase_gadget_fusion.
+  rewrite Z_phase_gadget_full_fusion.
   easy.
 Qed.
 
+Ltac crewrite H := rewrite H; clear H.
 
+Lemma cnot_commutes_through_phase_gadget : forall n α, 
+  (_NOTC_ ↕ n_wire _) ⟷ (— ↕ Z_phase_gadget (S n) α) ∝ (— ↕ Z_phase_gadget (S n) α) ⟷ (_NOTC_ ↕ n_wire _).
+Proof.
+  intros.
+  simpl.
+  destruct n.
+  - simpl. cleanup_zx. simpl_casts.
+    rewrite notc_is_notc_r.
+    rewrite ComposeRules.compose_assoc.
+    rewrite <- (stack_compose_distr — — (Z 2 1 0)).
+    assert (Z 2 1 0 ⟷ Z 1 1 α ∝ — ↕ Z 1 1 α ⟷ Z 2 1 0) as Hcomm.
+    {
+      rewrite <- Z_0_is_wire. 
+      rewrite <- Z_add_l.
+      rewrite Z_spider_1_1_fusion.
+      repeat rewrite Rplus_0_l.
+      easy.
+    } 
+    rewrite Hcomm.
+    cleanup_zx.
+    rewrite stack_wire_distribute_l.
+    rewrite <- (ComposeRules.compose_assoc (X 1 2 0 ↕ —)).
+    rewrite (stack_assoc_back — —).
+    simpl_casts.
+    rewrite <- (stack_compose_distr (X 1 2 0) (— ↕ —) — (Z 1 1 α)).
+    cleanup_zx.
+    rewrite <- (wire_removal_r (Z 1 1 α)).
+    rewrite stack_compose_distr.
+    rewrite <- (ComposeRules.compose_assoc).
+    rewrite <- (stack_compose_distr — (X 1 2 0)).
+    bundle_wires. cleanup_zx.
+    easy.
+  - simpl.
+    remember (Z_phase_gadget_construct n α) as pg.
+    rewrite wire_to_n_wire at 3.
+    rewrite n_wire_stack.
+    rewrite (@stack_nwire_distribute_r _ _ _ (1 + n)).
+    rewrite (ComposeRules.compose_assoc (— ↕ (Z 1 2 0) ↕ (n_wire (1 + n)))).
+    rewrite (stack_assoc (X 2 1 0) —).
+    simpl_casts.
+    bundle_wires.
+    rewrite <- (stack_compose_distr (X 2 1 0) — (n_wire (1 + (1 + n)))).
+    cleanup_zx.
+    rewrite <- nwire_removal_r.
+    rewrite (ComposeRules.compose_assoc (— ↕ (Z 1 2 0) ↕ (n_wire _)) (X 2 1 0 ↕ _) (n_wire (1 + (1 + (1 + n))))).
+    assert ((n_wire (1 + (1 + (1 + n)))) ∝ (— ↕ (— ↕ n_wire (1 + n)))) as Hrw by (bundle_wires; easy).
+    crewrite Hrw.
+    rewrite <- (stack_compose_distr (X 2 1 0) — ((Z 1 2 0 ↕ — ⟷ (— ↕ X 2 1 0) ↕ n_wire n ⟷ (— ↕ pg)
+      ⟷ (Z 1 2 0 ↕ — ⟷ (— ↕ X 2 1 0) ↕ n_wire n))) (— ↕ n_wire (1 + n))).
+    rewrite (wire_removal_r (X 2 1 0)).
+    rewrite <- (nwire_removal_l (X 2 1 0)) at 1.
+    rewrite (stack_compose_distr (n_wire 2)).
+    (* Move green spider *)
+    assert (n_wire 2 ∝ (— ↕ —)) as H2w by (bundle_wires; easy).
+    rewrite H2w at 1; clear H2w.
+    rewrite (stack_assoc — —).
+    rewrite stack_assoc.
+    simpl_casts.
+    rewrite <- (ComposeRules.compose_assoc (— ↕ (Z 1 2 0 ↕ n_wire (1 + n)))).
+    rewrite <- (stack_compose_distr — — (Z 1 2 0 ↕ n_wire (1 + n)) (— ↕ (Z 1 2 0 ↕ — ⟷ (— ↕ X 2 1 0) ↕ n_wire n ⟷ (— ↕ pg)
+      ⟷ (Z 1 2 0 ↕ — ⟷ (— ↕ X 2 1 0) ↕ n_wire n)))).
+    rewrite wire_removal_l.
+    rewrite (stack_wire_distribute_l (_CNOT_ ↕ n_wire _ ⟷ _)).
+    rewrite (stack_wire_distribute_l (_CNOT_ ↕ n_wire _)).
+    rewrite stack_nwire_distribute_r.
+    repeat rewrite (stack_wire_distribute_l (_ ↕ (n_wire n))). 
+    rewrite <- Z_0_is_wire at 3.
+    repeat rewrite <- ComposeRules.compose_assoc.
+    assert (Z 1 1 0 ↕ (Z 1 2 0 ↕ — ↕ n_wire n) ∝ ((Z 1 1 0 ↕ Z 1 2 0) ↕ (— ↕ n_wire n))) as Hstk.
+    {
+      repeat rewrite stack_assoc.
+      simpl_casts.
+      easy.
+    }
+    crewrite Hstk.
+    rewrite wire_to_n_wire at 3; rewrite n_wire_stack.
+    rewrite <- (@stack_nwire_distribute_r _ _ _ (1 + n) (Z 1 2 0) (Z 1 1 0 ↕ Z 1 2 0)). 
+    rewrite <- Z_add_r_base_rot.
+    repeat rewrite ComposeRules.compose_assoc.
+    rewrite (stack_wire_distribute_l (Z 1 2 0 ↕ — ↕ n_wire n) (— ↕ _ ↕ n_wire n)).
+    rewrite <- (ComposeRules.compose_assoc (— ↕ (— ↕ pg))).
+    rewrite (stack_assoc (Z 1 2 0) —).
+    simpl_casts.
+    rewrite <- stack_wire_distribute_l.
+    rewrite <- (stack_compose_distr — (Z 1 2 0) pg (— ↕ n_wire n)).
+    rewrite wire_removal_l.
+    rewrite <- (ComposeRules.compose_assoc (— ↕ (— ↕ X 2 1 0 ↕ n_wire n))).
+    rewrite <- stack_wire_distribute_l.
+    bundle_wires.
+    rewrite nwire_removal_r.
+    rewrite (stack_assoc — (X 2 1 0)).
+    simpl_casts.
+    rewrite <- (stack_compose_distr — (Z 1 2 0) (X 2 1 0 ↕ n_wire n) pg).
+    rewrite wire_removal_l.
+    rewrite <- (ComposeRules.compose_assoc (Z 1 (1 + 2) 0 ↕ n_wire (1 + n))).
+    rewrite (stack_assoc_back — (Z 1 2 0) (X 2 1 0 ↕ n_wire n ⟷ pg)).
+    simpl_casts.
+    rewrite <- Z_0_is_wire at 3.
+    rewrite <- (nwire_removal_l (X 2 1 0 ↕ n_wire n ⟷ pg)).
+    rewrite <- (nwire_removal_r (Z 1 1 0 ↕ Z 1 2 0)).
+    rewrite (stack_compose_distr (Z 1 1 0 ↕ Z 1 2 0)). 
+    rewrite <- (n_wire_stack 2 n).
+    rewrite <- (n_wire_stack 1 1).
+    rewrite (stack_assoc (n_wire 1) (n_wire 1) _).
+    simpl_casts.
+    rewrite (n_wire_stack 1 n).
+    rewrite stack_assoc_back.
+    simpl_casts.
+    repeat rewrite <- ComposeRules.compose_assoc.
+    rewrite <- (stack_nwire_distribute_r (Z 1 (1+2) 0) (Z 1 1 0 ↕ Z 1 2 0 ↕ n_wire 1 )).
+    rewrite (Z_add_r_base_rot 1 2).
+    rewrite stack_assoc.
+    simpl_casts.
+    rewrite Z_0_is_wire.
+    rewrite (ComposeRules.compose_assoc (Z 1 2 0)).
+    rewrite <- (stack_wire_distribute_l (Z 1 2 _) (Z 1 2 _ ↕ (n_wire 1))).
+    rewrite (dominated_Z_spider_fusion_top_left 2 0).
+    rewrite wire_to_n_wire at 2.
+    rewrite (dominated_Z_spider_fusion_bot_left 3 0 1).
+    rewrite 2 Rplus_0_l.
+    rewrite  (Z_add_r_base_rot 3 1).
+    rewrite Z_0_is_wire.
+    rewrite (stack_nwire_distribute_r (Z 1 2 0)).
+    rewrite (stack_assoc (Z 1 3 0)).
+    simpl_casts.
+    rewrite 3 ComposeRules.compose_assoc.
+    rewrite <- (ComposeRules.compose_assoc (Z 1 3 0 ↕ (— ↕ (n_wire _)))
+      (n_wire (1 + 2) ↕ (X 2 1 0 ↕ n_wire n ⟷ pg))).
+    rewrite <- (stack_compose_distr (Z 1 3 0) (n_wire 3) (— ↕ (n_wire (1+ n)))).
+    bundle_wires.
+    cleanup_zx.
+    rewrite <- (nwire_removal_l (Z 1 3 0)).
+    rewrite <- (nwire_removal_r (_ ⟷ pg)).
+    rewrite stack_compose_distr.
+    rewrite (Z_add_r_base_rot 2 1).
+    rewrite <- n_wire_stack.
+    rewrite stack_assoc_back.
+    simpl_casts.
+    rewrite (stack_nwire_distribute_l (X 2 1 0 ↕ n_wire n) pg).
+    rewrite (stack_nwire_distribute_r (Z 1 2 0)).
+    repeat rewrite stack_nwire_distribute_r.
+    repeat rewrite stack_wire_distribute_l.
+    repeat rewrite ComposeRules.compose_assoc.
+    rewrite <- wire_to_n_wire.
+    apply compose_simplify; [ easy | ].
+    apply compose_simplify; [
+    rewrite stack_assoc_back;
+    simpl_casts;
+    easy | ].
+    apply compose_simplify; [ easy | ].
+    rewrite <- (n_wire_stack 1 n).
+    rewrite <- wire_to_n_wire.
+    apply compose_simplify; [
+    rewrite (stack_assoc (Z 1 2 0) — (n_wire n));
+    simpl_casts;
+    easy | ].
+    rewrite Z_0_is_wire.
+    rewrite stack_assoc_back; simpl_casts.
+    rewrite <- ComposeRules.compose_assoc.
+    rewrite <- (stack_wire_distribute_l (Z 1 2 0 ↕ — ↕ (— ↕ n_wire n)) ((— ↕ — ↕ (X 2 1 0 ↕ n_wire n)))).
+    rewrite stack_assoc; simpl_casts.
+    rewrite <- (stack_compose_distr  (Z 1 2 0) (— ↕ —) (— ↕ (— ↕ n_wire n))).
+    rewrite wire_to_n_wire at 1 2 3 4 5.
+    repeat rewrite n_wire_stack.
+    rewrite nwire_removal_l.
+    rewrite nwire_removal_r.
+    rewrite <- (wire_removal_l (Z 1 2 0)) at 1.
+    rewrite <- (wire_removal_r (X 2 1 0)) at 1.
+    rewrite (stack_assoc_back (— ⟷ Z 1 2 0) (X 2 1 0 ⟷ —) (n_wire n)); simpl_casts.
+    rewrite stack_compose_distr.
+    rewrite stack_nwire_distribute_r, stack_nwire_distribute_l.
+    rewrite ComposeRules.compose_assoc.
+    rewrite <- wire_to_n_wire.
+    apply compose_simplify; [ easy | ].
+    bundle_wires.
+    rewrite stack_nwire_distribute_r.
+    apply compose_simplify.
+    + rewrite stack_assoc; simpl_casts.
+      bundle_wires.
+      rewrite (stack_assoc — (Z 1 2 0) (n_wire _)); simpl_casts.
+      easy.
+    + rewrite (stack_assoc (X 2 1 0) — (n_wire _)); simpl_casts.
+      bundle_wires.
+      easy.
+Unshelve.
+  all: lia.
+Qed.
+
+
+
+
+
+    
+
+
+    
+
+    
+    
+    
+    
+    
+
+
+      
+    
